
$$
\begin{equation}
X_{1}a + X_{2}b = PX
\end{equation}
$$

$$
b = \frac{PX-X_{1}a}{X_{2}}
$$
$$
Y_{1}a + Y_{2}b = PY
$$
$$
a = \frac{PY-Y_{2}b}{Y_{1}}
$$


then sub into (2) into (1)

(1) becomes:
$$
b = \frac{PX - X_{1}(\frac{PY-Y_{2}b}{Y_{1}})}{X_{2}}
$$
then we can multiply out to get b on the same side:

$$
b*X_{2} = PX - X_{1}(\frac{PY-Y_{2}b}{Y_{1}})
$$
simplify further
$$
 Y_{1}(b*X_{2}-PX)=-X_{1}PY+X_{1}Y_{2}b
$$
$$
bY_{1}X_{2}-Y_{1}PX = -X_{1}PY + bX_{1}Y_{2}
$$
$$
bY_{1}X_{2}-bX_{1}Y_{2} = -X_{1}PY+Y_{1}PX
$$
$$
b = \frac{-X_{1}PY + Y_{1}PX}{Y_{1}X_{2}-X_{1}Y_{2}}
$$

once we find b we can find a with:

$$
a = \frac{PY-Y_{2}b}{Y_{1}}
$$
